Continue rewriting into Lean4
Rewrite:
- TreeSet
- TreeMap
- bool_reflect tactic
- definition of Graph

TODO Fix LinearOrder on Edge

src/hog/Graph.lean
@@ -1,6 +1,63 @@
+import Mathlib.Order.Basic
 import Mathlib.Order.Synonym
+import Mathlib.Data.Prod.Lex
+import Init.Prelude
+import TreeSet
+import TreeMap
+import Tactic
+
+open TreeSet
+open TreeMap
 
 -- The type of edges
-structure edge : Type :=
-  (edge : Lex (Nat × Nat))
-  (src_lt_trg : edge.fst < edge.snd)
+structure Edge : Type :=
+  edge        : Lex (Nat × Nat)
+  src_lt_trg  : edge.fst < edge.snd := by bool_reflect
+
+instance EdgeLinearOrder : LinearOrder Edge := 
+  LinearOrder.lift' (fun (u : Edge) => u.edge) (fun u v H => by cases u; cases v; simp; assumption)
+
+-- def nbhds_condition (nbhds : tmap ℕ (tset ℕ)) : Prop :=
+--   ∀ i : ℕ, smap.contains_key i nbhds → (∀ j : ℕ, j ∈ nbhds.to_map i → i ∈ nbhds.to_map j)
+
+-- theorem test (nbhds : Tmap ℕ (Tset ℕ)) : DecidablePred (fun j => i ∈ nbhds.toMap j) := by
+--   intro j
+
+def decidableNbhdsCondition (nbhds : Tmap ℕ (Tset ℕ)) : Bool := sorry
+  -- Smap.forallKeys (fun i => Stree.optionForall (fun j => i ∈ nbhds.toMap j) (nbhds.toMap i)) nbhds
+
+-- def nbhds_describe_edges (nbhds : tmap ℕ (tset ℕ)) (edges : tset edge) : Prop := 
+--   ∀ i : ℕ, smap.contains_key i nbhds → (∀ j : ℕ, j ∈ nbhds.to_map i → decidable.lt_by_cases i j
+--     (λ _, {edge . edge := (i, j)} ∈ edges)
+--     (λ _, false)
+--     (λ _, {edge . edge := (j, i)} ∈ edges))
+
+-- def decidable_nbhds_describe_edges (nbhds : tmap ℕ (tset ℕ)) (edges : tset edge) : bool := 
+--   smap.forall_keys (λ i, (@stree.option_forall ℕ (_) (λ j, 
+--     decidable.lt_by_cases i j
+--       (λ _, {edge . edge := (i, j)} ∈ edges)
+--       (λ _, false)
+--       (λ _, {edge . edge := (j, i)} ∈ edges))
+--     ) (begin simp [decidable.lt_by_cases], apply_instance end) (_) (_) (_) (nbhds.to_map i)) nbhds
+
+-- def edges_describe_nbhds (nbhds : tmap ℕ (tset ℕ)) (edges : tset edge) : Prop :=
+--   ∀ e : edge, e ∈ edges → e.edge.snd ∈ nbhds.to_map e.edge.fst
+
+-- def decidable_edges_describe_nbhds (nbhds : tmap ℕ (tset ℕ)) (edges : tset edge) : bool :=
+--   stree.forall (λ e : edge, e.edge.snd ∈ nbhds.to_map e.edge.fst) edges
+
+-- def describes_neighborhoods (nbhds : tmap ℕ (tset ℕ)) (edges : tset edge) : Prop := 
+-- nbhds_condition nbhds ∧ nbhds_describe_edges nbhds edges ∧ edges_describe_nbhds nbhds edges
+
+-- def decidable_describes_neighborhoods (nbhds : tmap ℕ (tset ℕ)) (edges : tset edge) : bool := 
+-- decidableNbhdsCondition nbhds ∧ decidable_nbhds_describe_edges nbhds edges ∧ decidable_edges_describe_nbhds nbhds edges
+
+-- The definition of a finite graph that will represent the graphs that we import from House of Graphs
+
+structure SimpleIrreflexiveGraph : Type :=
+  (vertexSize : ℕ)
+  (edges : Tset Edge)
+  (edgeSize : ℕ)
+  (edgeSizeCorrect : edgeSize = edges.size)
+  (neighborhoods : Tmap ℕ (Tset ℕ))
+  (neighborhoods_correct : decidableNbhdsCondition neighborhoods = tt)
