lakefile.lean
@@ -5,9 +5,10 @@ package «lean-HOG» {
   srcDir := "src/hog"
 }
 
-lean_lib TreeSet {
-}
+lean_lib TreeSet
 lean_lib TreeMap
+lean_lib Graph
+lean_lib Tactic
 
 require mathlib from git
   "https://github.com/leanprover-community/mathlib4.git"
