src/hog/ExampleData.lean
@@ -1,0 +1,140 @@
+-- import Mathlib.Init.Data.Bool.Lemmas
+import Graph
+import TreeSet
+import TreeMap
+import Tactic
+
+namespace hog
+
+open TreeSet
+open TreeMap
+open Tactic
+
+def edge_1 : Edge := { edge := (0,2), src_lt_trg := by trivial }
+def edge_2 : Edge := { edge := (0,1), src_lt_trg := by trivial }
+
+
+instance compareEdgeDecidable (e1 e2 : Edge) : Decidable (e1 < e2) := by
+  have l : LinearOrder Edge := by apply EdgeLinearOrder
+  have r := l.decidable_lt
+  have q := r e1 e2
+  simp at q
+  -- exact q
+  sorry
+
+set_option pp.analyze.checkInstances true in
+lemma foo :  ({ edge := (0,2), src_lt_trg := by trivial } : Edge) < ({ edge := (0,1), src_lt_trg := by trivial }: Edge) := by
+  have l : LinearOrder Edge := by apply EdgeLinearOrder
+  apply Bool.of_decide_true
+  sorry
+
+  
+def example_1: Tset Edge :=
+  Stree.node { edge := (0,2) }
+    (Stree.leaf { edge := (0,1) } (by trivial) (by sorry))
+    (Stree.leaf { edge := (1,2) } (by sorry) (by sorry))
+
+def temp0 : tset ℕ :=
+  stree.node 1
+    (stree.empty (by bool_reflect))
+    (stree.leaf 2 (by bool_reflect) (by bool_reflect))
+
+def temp1 : tset ℕ :=
+  stree.node 0
+    (stree.empty (by bool_reflect))
+    (stree.leaf 2 (by bool_reflect) (by bool_reflect))
+
+def temp2 : tset ℕ :=
+  stree.node 0
+    (stree.empty (by bool_reflect))
+    (stree.leaf 1 (by bool_reflect) (by bool_reflect))
+
+def N₁ : tmap ℕ (tset ℕ) :=
+  smap.node 1 temp1
+    (smap.leaf 0 temp0 (by bool_reflect) (by bool_reflect))
+    (smap.leaf 2 temp2 (by bool_reflect) (by bool_reflect))
+
+
+def g : simple_irreflexive_graph := 
+{ vertex_size := 3,
+  edges := example_1,
+  edge_size := 3,
+  edge_size_correct := by refl,
+  neighborhoods := N₁,
+  neighborhoods_correct := by refl
+}
+
+def w : num_components_witness := { 
+  G := g,
+  num_components := 1,
+  c := λ v : ℕ, 
+    match v with
+    | 0 := 0
+    | 1 := 0
+    | 2 := 0
+    | _ := 0
+    end,
+  h := λ v, 
+    match v with
+    | 0 := 0
+    | 1 := 1
+    | 2 := 2
+    | _ := 0
+    end,
+  connect_edges := 
+    begin 
+      apply tset.forall_is_forall,
+      bool_reflect
+    end,
+  root := λ (v : fin 1),
+    match v with
+    | ⟨ 0, _ ⟩ := 0
+    | _ := 0
+    end,
+  is_root := λ i,
+    match i with
+    | ⟨ 0, _ ⟩ := by bool_reflect
+    | i := sorry
+    end,
+  uniqueness_of_roots := λ v,
+    match v with
+    | 0 := by bool_reflect
+    | 1 := by contradiction
+    | 2 := by contradiction
+    | _ := sorry
+    end,
+  next := λ v,
+    match v with
+    | 0 := 0
+    | 1 := 0
+    | 2 := 1
+    | _ := 0
+    end,
+  height_cond := λ v,
+    match v with
+    | 0 := 
+      begin
+        have nh : ¬ 0 < 0 := irrefl 0,
+        contradiction
+      end
+    | 1 := 
+      begin 
+        intro h,
+        simp [edge_relation, decidable.lt_by_cases],
+        bool_reflect
+      end
+    | 2 :=
+      begin 
+        intro h,
+        simp [edge_relation, decidable.lt_by_cases],
+        bool_reflect
+      end
+    | _ := sorry
+    end
+}
+
+def wc : number_of_connected_components := witness_components w
+
+
+end hog
+
