src/hog/Tactic.lean
@@ -1,0 +1,11 @@
+import Mathlib.Init.Data.Bool.Lemmas
+
+namespace LeanHog.Tactic
+
+open Lean Elab.Tactic Parser.Tactic Lean.Meta
+
+syntax "bool_reflect" : tactic
+macro_rules
+| `(tactic| bool_reflect) => `(tactic| apply Bool.of_decide_true; rfl)
+
+end LeanHog.Tactic
